WIP on proof

SyMac/SMSemantics.v
@@ -28,43 +28,53 @@ Module Type SMSEMANTICS
   Definition env := PM.t value.
   Definition history := PM.t (stream value).
 
-  Definition memory := RMemory.memory (list value).
-  Definition memories := RMemory.memory (list (stream value)).
+  Record mvalues :=
+    { first: stream value;
+      inter: list (stream value)
+      (* last : stream value *)
+    }.
 
-  Fixpoint find_init (x: ident) (mems: list (ident * const)): option value :=
+  Record mvalue :=
+    { first_i: value;
+      inter_i: list value
+      (* last_i : value *)
+    }.
+
+  Definition memory := RMemory.memory mvalue.
+  Definition memories := RMemory.memory mvalues.
+
+  Fixpoint find_init (x: ident) (mems: list (ident * const)): option const :=
     match mems with
     | [] => None
     | m :: mems =>
       if ident_eqb (fst m) x
-      then Some (present (sem_const (snd m))) else find_init x mems
+      then Some (snd m) else find_init x mems
     end.
 
-  Definition get_mem (k: nat) (init: bool) (x: ident) (m: memory) (mems: list (ident * const)):=
-    if init then find_init x mems
-    else match mfind_mem x m with
-         | Some lv =>
-           match k with
-           | 0 => nth_error lv 0
-           | S k' =>
-             match nth_error lv k' with
-             | Some absent => nth_error lv k
-             | None => None
-             | v => v
-             end
-           end
-         | None => None
-         end.
+  Fixpoint get_last (first: value) (inter: list value): value :=
+    match inter with
+    | [] => first
+    | absent :: vs => get_last first vs
+    | present v :: _ => present v
+    end.
+
+  Definition get_mem (* (init: bool) *) (x: ident) (m: memory) (* (mems: list (ident * const)) *) :=
+    (* if init then find_init x mems else *)
+      match mfind_mem x m with
+      | Some mv => Some (get_last mv.(first_i) mv.(inter_i))
+      | None => None
+      end.
 
   (** ** Instantaneous semantics *)
 
   Section InstantSemantics.
 
-    Variable init: bool.
+    (* Variable init: bool. *)
     Variable base: bool.
     Variable R: env.
     Variable m: memory.
-    Variable k: nat.
-    Variable mems: list (ident * const).
+    (* Variable k: rank. *)
+    (* Variable mems: list (ident * const). *)
 
     Inductive sem_var_instant: ident -> value -> Prop :=
       Sv:
@@ -75,7 +85,7 @@ Module Type SMSEMANTICS
     Inductive sem_mem_var_instant: ident -> value -> Prop :=
       Smv:
         forall x v,
-          get_mem k init x m mems = Some v ->
+          get_mem (* init *) x m (* mems *) = Some v ->
           sem_mem_var_instant x v.
 
     Inductive sem_clock_instant: clock -> bool -> Prop :=
@@ -215,24 +225,24 @@ Module Type SMSEMANTICS
   End InstantSemantics.
 
   Section InstantAnnotatedSemantics.
-    Variable init : bool.
+    (* Variable init : bool. *)
     Variable base : bool.
     Variable R: env.
     Variable m: memory.
-    Variable k: nat.
-    Variable mems: list (ident * const).
+    (* Variable k: rank. *)
+    (* Variable mems: list (ident * const). *)
 
     Inductive sem_annotated_instant {A}
-              (sem_instant: bool -> bool -> env -> memory -> nat -> list (ident * const) -> A -> value -> Prop)
+              (sem_instant: bool -> (* bool -> *) env -> memory -> (* list (ident * const) -> *) A -> value -> Prop)
       : clock -> A -> value -> Prop :=
     | Stick:
         forall ck a c,
-          sem_instant init base R m k mems a (present c) ->
+          sem_instant (* init *) base R m (* mems *) a (present c) ->
           sem_clock_instant base R ck true ->
           sem_annotated_instant sem_instant ck a (present c)
     | Sabs:
         forall ck a,
-          sem_instant init base R m k mems a absent ->
+          sem_instant (* init *) base R m (* mems *) a absent ->
           sem_clock_instant base R ck false ->
           sem_annotated_instant sem_instant ck a absent.
 
@@ -243,13 +253,13 @@ Module Type SMSEMANTICS
     | SLticks:
         forall ck ces cs vs,
           vs = map present cs ->
-          sem_lexps_instant init base R m k mems ces vs ->
+          sem_lexps_instant (* init *) base R m (* mems *) ces vs ->
           sem_clock_instant base R ck true ->
           sem_laexps_instant ck ces vs
     | SLabss:
         forall ck ces vs,
           vs = all_absent ces ->
-          sem_lexps_instant init base R m k mems ces vs ->
+          sem_lexps_instant (* init *) base R m (* mems *) ces vs ->
           sem_clock_instant base R ck false ->
           sem_laexps_instant ck ces vs.
 
@@ -262,20 +272,20 @@ Module Type SMSEMANTICS
     Variable bk : stream bool.
     Variable H : history.
     Variable M: memories.
-    Variable k: nat.
-    Variable mems: list (ident * const).
+    (* Variable k: rank. *)
+    (* Variable mems: list (ident * const). *)
 
     Definition restr_hist (n: nat): env :=
       PM.map (fun xs => xs n) H.
     Hint Unfold restr_hist.
 
     Definition restr_mem (n: nat): memory :=
-      mmap (fun lv => map (fun xs => xs n) lv) M.
+      mmap (fun mv => {| first_i := mv.(first) n; inter_i := map (fun vs => vs n) mv.(inter) |}) M.
     Hint Unfold restr_mem.
 
-    Definition lift {A B} (sem: bool -> bool -> env -> memory -> nat -> list (ident * const) -> A -> B -> Prop)
+    Definition lift {A B} (sem: (* bool -> *) bool -> env -> memory -> (* list (ident * const) -> *) A -> B -> Prop)
                x (ys: stream B): Prop :=
-      forall n, sem (n ==b 0) (bk n) (restr_hist n) (restr_mem n) k mems x (ys n).
+      forall n, sem (* (n ==b 0) *) (bk n) (restr_hist n) (restr_mem n) (* mems *) x (ys n).
     Hint Unfold lift.
 
     Definition lift' {A B} (sem: bool -> env -> A -> B -> Prop) x (ys: stream B): Prop :=
@@ -296,10 +306,10 @@ Module Type SMSEMANTICS
       lift'' (fun R => Forall2 (sem_var_instant R)) x xs.
 
     Definition sem_laexp ck (e: lexp) (xs: stream value): Prop :=
-      lift (fun init base R m k mems => sem_laexp_instant init base R m k mems ck) e xs.
+      lift (fun (* init *) base R m (* mems *) => sem_laexp_instant (* init *) base R m (* mems *) ck) e xs.
 
     Definition sem_laexps (ck: clock) (e: list lexp) (xs: stream (list value)): Prop :=
-      lift (fun init base R m k mems => sem_laexps_instant init base R m k mems ck) e xs.
+      lift (fun (* init *) base R m (* mems *) => sem_laexps_instant (* init *) base R m (* mems *) ck) e xs.
 
     Definition sem_lexp (e: lexp) (xs: stream value): Prop :=
       lift sem_lexp_instant e xs.
@@ -308,7 +318,7 @@ Module Type SMSEMANTICS
       lift sem_lexps_instant e xs.
 
     Definition sem_caexp ck (c: cexp) (xs: stream value): Prop :=
-      lift (fun init base R m k mems => sem_caexp_instant init base R m k mems ck) c xs.
+      lift (fun (* init *) base R m (* mems *) => sem_caexp_instant (* init *) base R m (* mems *) ck) c xs.
 
     Definition sem_cexp (c: cexp) (xs: stream value): Prop :=
       lift sem_cexp_instant c xs.
@@ -347,40 +357,53 @@ Module Type SMSEMANTICS
   (*     apply H; eauto. *)
   (* Qed. *)
 
-  Inductive post_mem: nat -> ident -> stream value -> memories -> Prop :=
-    next_mem_intro:
-      forall k x xs M lvs lv,
-        mfind_mem x M = Some lvs ->
-        nth_error lvs k = Some lv ->
-        (forall n, lv (S n) = xs n) ->
-        post_mem k x xs M.
+  Inductive post_mem: rank -> ident -> stream value -> memories -> list (ident * const) -> Prop :=
+  (* | post_mem_first: *)
+  (*     forall x xs M mvs vs, *)
+  (*       mfind_mem x M = Some mvs -> *)
+  (*       hd_error mvs.(inter) = Some vs -> *)
+  (*       xs ≈ vs -> *)
+  (*       post_mem (Inter 0) x xs M *)
+  | post_mem_inter:
+      forall k x xs M mems mvs vs,
+        mfind_mem x M = Some mvs ->
+        nth_error mvs.(inter) k = Some vs ->
+        xs ≈ vs ->
+        post_mem (Inter k) x xs M mems
+  | post_mem_last:
+      forall x xs M mems mvs c0,
+        mfind_mem x M = Some mvs ->
+        find_init x mems = Some c0 ->
+        mvs.(first) ≈ fby (sem_const c0) xs ->
+        (* (forall n, mvs.(first) (S n) = xs n) -> *)
+        post_mem Last x xs M mems.
 
   Section ModeSemantics.
 
     Variable P: program.
 
-    Inductive sem_equation: nat -> stream bool -> history -> memories -> list (ident * const) -> equation -> Prop :=
+    Inductive sem_equation: rank -> stream bool -> history -> memories -> list (ident * const) -> equation -> Prop :=
     | SEqDef:
         forall k bk H M mems x xs ck ce,
           sem_var H x xs ->
-          sem_caexp bk H M k mems ck ce xs ->
+          sem_caexp bk H M (* mems *) ck ce xs ->
           sem_equation k bk H M mems (EqDef x ck ce)
     | SEqPost:
         forall k bk H M mems x ck ce xs,
-          sem_caexp bk H M k mems ck ce xs ->
-          post_mem k x xs M ->
+          sem_caexp bk H M (* mems *) ck ce xs ->
+          post_mem k x xs M mems ->
           sem_equation k bk H M mems (EqPost x ck ce)
     | SEqCall:
         forall k bk H M mems ys x Mx ck ma_n P' ma i m k' es ess oss,
           find_machine ma_n P = Some (ma, P') ->
-          sem_laexps bk H M k mems ck es ess ->
+          sem_laexps bk H M (* mems *) ck es ess ->
           hd_error ys = Some x ->
           sub_inst x M Mx ->
           sem_mode k' ma m Mx ess oss ->
           sem_vars H ys oss ->
           sem_equation k bk H M mems (EqCall ys ck ma_n i m k' es)
 
-    with sem_mode: nat -> machine -> ident -> memories -> stream (list value) -> stream (list value) -> Prop :=
+    with sem_mode: rank -> machine -> ident -> memories -> stream (list value) -> stream (list value) -> Prop :=
            SMode:
              forall k ma mo mo_n M H xss yss bk,
                clock_of xss bk ->
