NLustreToSyMac/Correctness.v
@@ -11,14 +11,15 @@ Require Import Velus.NLustre.Stream.
 Require Import Velus.NLustre.NLSemantics.
 Require Import Velus.SyMac.SMSemantics.
 Require Import Velus.NLustreToSyMac.Translation.
+Require Import Velus.RMemory.
 
 Require Import List.
 Import List.ListNotations.
 Require Import Coq.Sorting.Permutation.
 Require Import Morphisms.
 
-Open Scope positive.
 Open Scope list.
+Open Scope nat.
 
 Module Type CORRECTNESS
        (Import Ids   : IDS)
@@ -34,8 +35,14 @@ Module Type CORRECTNESS
        (Import Mem   : MEMORIES    Ids Op       Clks SynNL)
        (Import Trans : TRANSLATION Ids Op       Clks SynNL SynSM Mem).
 
-  Definition memory_spec (m: SemSM.memory) (mems: list (ident * const)) x :=
-    PS.mem x (ps_from_list (map fst mems)) = true <-> exists lv, RMemory.mfind_mem x m = Some lv.
+  Definition memory_spec (m: SemSM.memory) (memids: PS.t) (R: env) :=
+    forall x v,
+      PM.find x R = Some v ->
+      PS.mem x memids = true ->
+      SemSM.get_mem x m = Some v.
+
+  Definition memories_spec (M: SemSM.memories) (memids: PS.t) (H: history) :=
+    forall n, memory_spec (SemSM.restr_mem M n) memids (SemSM.restr_hist H n).
 
   Section Global.
 
@@ -64,31 +71,33 @@ Module Type CORRECTNESS
         induction 1; eauto using SemSM.sem_clock_instant.
       Qed.
 
+      Variable m: SemSM.memory.
+      Variable memids: PS.t.
+      Hypothesis Spec: memory_spec m memids R.
+      (* Variable mems: list (ident * const). *)
+      (* Let memids := ps_from_list (map fst mems). *)
+
       Lemma typeof_correctness:
-        forall e mems,
-          SynSM.typeof (translate_lexp mems e) = typeof e.
+        forall e,
+          SynSM.typeof (translate_lexp memids e) = typeof e.
       Proof.
         induction e; intros; simpl; auto.
-        destruct (PS.mem i mems); auto.
+        destruct (PS.mem i memids); auto.
       Qed.
       (* Hint Resolve typeof_correctness. *)
 
-      Variable m: SemSM.memory.
-      Variable mems: list (ident * const).
-      Let memids := ps_from_list (map fst mems).
-
       Lemma lexp_instant_correctness:
-        forall e b v,
+        forall e v,
           sem_lexp_instant base R e v ->
-          SemSM.sem_lexp_instant b base R m 0 mems (translate_lexp memids e) v.
+          SemSM.sem_lexp_instant base R m (translate_lexp memids e) v.
       Proof.
         induction 1; simpl; eauto using SemSM.sem_lexp_instant.
         - destruct (PS.mem x memids) eqn: E.
           + do 2 constructor.
             unfold SemSM.get_mem.
-            destruct b.
-            * admit.
-            * admit.
+            match goal with H: sem_var_instant R x v |- _ =>
+                            inversion_clear H as [?? Find] end.
+            apply Spec; auto.
           + eauto using SemSM.sem_lexp_instant.
         - econstructor; eauto.
           now rewrite typeof_correctness.
@@ -98,17 +107,17 @@ Module Type CORRECTNESS
       Hint Resolve lexp_instant_correctness.
 
       Lemma lexps_instant_correctness:
-        forall es b vs,
+        forall es vs,
           sem_lexps_instant base R es vs ->
-          SemSM.sem_lexps_instant b base R m 0 mems (map (translate_lexp memids) es) vs.
+          SemSM.sem_lexps_instant base R m (map (translate_lexp memids) es) vs.
       Proof.
         induction 1; constructor; auto.
       Qed.
 
       Lemma cexp_instant_correctness:
-        forall ce b v,
+        forall ce v,
           sem_cexp_instant base R ce v ->
-          SemSM.sem_cexp_instant b base R m 0 mems (translate_cexp memids ce) v.
+          SemSM.sem_cexp_instant base R m (translate_cexp memids ce) v.
       Proof.
         induction 1; simpl; eauto using SemSM.sem_cexp_instant.
       Qed.
@@ -142,36 +151,55 @@ Module Type CORRECTNESS
       Qed.
 
       Variable M: SemSM.memories.
-      Variable mems: list (ident * const).
-      Let memids := ps_from_list (map fst mems).
+      Variable memids: PS.t.
+      Hypothesis Spec: memories_spec M memids H.
+      (* Variable mems: list (ident * const). *)
+      (* Let memids := ps_from_list (map fst mems). *)
+
+      Lemma laexp_correctness:
+        forall ck e xs,
+          sem_laexp bk H ck e xs ->
+          SemSM.sem_laexp bk H M ck (translate_lexp memids e) xs.
+      Proof.
+        intros ** Sem n; specialize (Sem n); simpl in Sem.
+        induction Sem; constructor; auto.
+      Qed.
 
       Lemma caexp_correctness:
         forall ck ce xs,
           sem_caexp bk H ck ce xs ->
-          SemSM.sem_caexp bk H M 0 mems ck (translate_cexp memids ce) xs.
+          SemSM.sem_caexp bk H M ck (translate_cexp memids ce) xs.
       Proof.
         intros ** Sem n; specialize (Sem n); simpl in Sem.
-        induction Sem; constructor; auto;
-          apply cexp_instant_correctness; auto.
+        induction Sem; constructor; auto.
       Qed.
 
       Lemma laexps_correctness:
         forall ck es vs,
           sem_laexps bk H ck es vs ->
-          SemSM.sem_laexps bk H M 0 mems ck (map (translate_lexp memids) es) vs.
+          SemSM.sem_laexps bk H M ck (map (translate_lexp memids) es) vs.
       Proof.
         intros ** Sem n; specialize (Sem n); simpl in Sem.
         induction Sem.
         - econstructor 1; eauto.
-          now apply lexps_instant_correctness.
         - constructor; auto.
-          + now rewrite all_absent_map.
-          + now apply lexps_instant_correctness.
+          now rewrite all_absent_map.
+      Qed.
+
+      Lemma sem_caexp_laexp:
+        forall ck e xs,
+          SemSM.sem_caexp bk H M ck (SynSM.Eexp e) xs
+          <-> SemSM.sem_laexp bk H M ck e xs.
+      Proof.
+        split; intros ** Sem n; specialize (Sem n).
+        - inv Sem; match goal with H: SemSM.sem_cexp_instant _ _ _ _ _ |- _ => inv H end;
+            constructor; auto.
+        - induction Sem; repeat constructor; auto.
       Qed.
 
     End Sem.
     Hint Resolve var_correctness vars_correctness
-         caexp_correctness laexps_correctness.
+         laexp_correctness caexp_correctness laexps_correctness.
 
 
     Theorem correctness:
@@ -179,25 +207,22 @@ Module Type CORRECTNESS
         sem_node G f xss oss ->
         exists ma,
           (forall n, find_node f G = Some n -> ma = translate_node n)
-          /\ exists M, SemSM.sem_mode P 0 ma step M xss oss.
+          /\ exists M, SemSM.sem_mode P SynSM.Last ma step M xss oss.
     Proof.
       induction 1 as [| | | |???? IHNode|] using sem_node_mult with
           (P_equation := fun b H e =>
                            sem_equation G b H e ->
                            exists M mems,
-                             Forall (SemSM.sem_equation P 0 b H M mems)
+                             Forall (SemSM.sem_equation P SynSM.Last b H M mems)
                                     (translate_eqn (ps_from_list (map fst mems)) e))
           (P_reset := fun f r xss oss =>
                         sem_reset G f r xss oss ->
                         True);
         eauto.
       - repeat (econstructor; eauto).
+        apply caexp_correctness; auto.
 
       - intro Sem; clear Sem.
-        (* match goal with *)
-        (*   H: sem_node _ _ _ _ |- _ => *)
-        (*   inversion_clear H as [??????? Find] *)
-        (* end. *)
         destruct IHsem_node as (ma & Spec & M & Sem).
         match goal with
           H: sem_node _ _ _ _ |- _ =>
@@ -207,24 +232,39 @@ Module Type CORRECTNESS
         apply Spec in Find'.
         apply find_node_translate in Find as (ma' & ? & Find & E).
         subst.
-        (* apply find_node_translate in Find. *)
-        (* destruct Find as (ma' & P' & Find' & E). *)
-
         simpl.
-        do 2 econstructor.
-        constructor; eauto.
+        assert (exists y, hd_error x = Some y) as (y & ?).
+        { apply length_hd_error.
+          repeat match goal with H: sem_vars _ _ _ _ |- _ => specialize (H 0); simpl in H end.
+          repeat match goal with H: Forall2 _ _ _ |- _ => apply Forall2_length in H end.
+          match goal with H: length x = _ |- _ => rewrite H end.
+          repeat try match goal with H: _ = ?x |- _ => rewrite <-H end.
+          rewrite map_length; apply n.(n_outgt0).
+        }
+        exists (madd_obj y M (@empty_memory SemSM.mvalues)).
+        repeat (econstructor; eauto).
+        apply mfind_inst_gss.
+
+      - admit.
+
+      - intro Sem; clear Sem; simpl.
+        exists (madd_mem x {| SemSM.first := xs; SemSM.inter := [] |} (@empty_memory SemSM.mvalues)).
+        exists [(x, c0)].
         econstructor; eauto.
-        +
-          SearchAbout SynSM.find_machine.
-
-
-  sem_det. admit.
-
-      - admit.
-
-      - admit.
-
-      - admit.
+        econstructor; eauto.
+        + apply sem_caexp_laexp; eauto.
+        + econstructor.
+          * apply mfind_mem_gss.
+          * simpl; now rewrite ident_eqb_refl.
+          * simpl; intro n.
+            match goal with H: xs = _ |- _ => now rewrite H end.
 
       - exists (translate_node n); split; eauto.
+        + intros.
+          match goal with
+          | H: find_node ?f ?G = Some _,
+               H': find_node f G = Some _ |- _ => rewrite H in H'; inv H'
+          end; auto.
+        +
+
     Qed.
